Updates

high2/Zeta.EAC.fst
@@ -1,6 +1,85 @@
 module Zeta.EAC
 
+open Zeta.SeqMachine
 open Zeta.SeqAux
+
+let eac_state_of_base_key
+  (#app: app_params)
+  (l: vlog_ext app)
+  (k: base_key): eac_state app k
+  = seq_machine_run (eac_smk app k) l
+
+let eac_state_transition_aux
+  (#app: app_params)
+  (l: vlog_ext app {length l > 0})
+  (k: base_key)
+  : Lemma (ensures (let open Zeta.SeqAux in
+                    let n = length l - 1 in
+                    let l' = prefix l n in
+                    let ee = index l n in
+                    let es' = eac_state_of_base_key l' k in
+                    let es = eac_state_of_base_key l k in
+                    es = eac_add ee es'))
+          [SMTPat (eac_state_of_base_key l k)]
+  = admit()
+
+let eac_state_transition
+  (#app: app_params)
+  (l: vlog_ext app {length l > 0})
+  (k: key app)
+  : Lemma (ensures (let open Zeta.SeqAux in
+                    let n = length l - 1 in
+                    let l' = prefix l n in
+                    let ee = index l n in
+                    let es' = eac_state_of_key l' k in
+                    let es = eac_state_of_key l k in
+                    es = eac_add ee es'))
+  =
+
+  admit()
+
+let eac_empty_log
+  (#app: app_params)
+  (l: vlog_ext app {length l = 0})
+  : Lemma (ensures (eac l))
+          [SMTPat (eac l)]
+  = admit()
+
+let eac_induction_step_helper
+  (#app: app_params)
+  (l: vlog_ext app)
+  (i: seq_index l {eac (prefix l i)})
+  : o: (option base_key)
+    {
+      o = None /\ eac (prefix l (i + 1))
+          \/
+      (let k = Some?.v o in
+       eac_state_of_key (prefix l (i + 1)) k = EACFail)
+    }
+  = admit()
+
+let rec max_eac_prefix_aux
+  (#app: app_params)
+  (l:vlog_ext app)
+  : Tot (ki: (base_key & nat) {
+      let k,i = ki in
+      eac l /\ i = length l
+          \/
+      i < length l /\
+      eac (prefix l i) /\
+      ~ (eac (prefix l (i + 1))) /\
+      ~ (valid (eac_smk app k) (prefix l (i + 1)))
+      })
+     (decreases (length l))
+  = let n = length l in
+    if n = 0 then Zeta.BinTree.Root (* any key since eac*), 0
+    else
+      let n = n - 1 in
+      let l' = prefix l n in
+      let ee = index l n in
+      let i' = max_eac_prefix_aux l' in
+      admit()
+
 
 let eac_implies_prefix_eac
   (#app: app_params)
